add byte level splitting

include/smack/BlockExecutor.h
@@ -59,6 +59,8 @@ namespace smack{
 
         SHExprPtr executeMalloc(SHExprPtr sh, const CallStmt* stmt);
 
+        SHExprPtr executeAlloca(SHExprPtr sh, const Stmt* stmt);
+
         SHExprPtr executeFree(SHExprPtr sh, const CallStmt* stmt);
 
         SHExprPtr executeCast(SHExprPtr sh, const Stmt* stmt);
