include/utils/TranslatorUtil.h
@@ -15,8 +15,8 @@ namespace smack
         TranslatorUtil(/* args */){};
         ~TranslatorUtil(){};
         static z3::expr getBase(int index, z3::context& ctx);
-        
-    
+        static z3::expr byteVarSizeConstraint(std::string varName, int byteIndex, z3::context& z3Ctx);
+        static z3::expr splitLargeVariable(std::string varName, int byteIndex, z3::context& z3Ctx);
     };
 
 
