testcases/printtest/exec.bpl
@@ -6,12 +6,48 @@ axiom (main == $sub.ref(0, 1032));
 procedure {:entrypoint} main()
   returns ($r: i32)
 {
-  var $p0: ref8;
-  var $p1: ref32;
+  var $p0: ref;
+  var $p1: ref8;
+  var $p2: ref;
+  var $p3: ref8;
+  var $p4: ref;
+  var $p5: ref;
+  var $p6: ref8;
+  var $p7: ref;
+  var $p8: ref8;
+  var $i9: i1;
+  var $p10: ref;
+  var $p11: ref;
 $bb0:
   call {:cexpr "smack:entry:main"} boogie_si_record_ref(main);
-  call $p0 := malloc(1);
-  $p1 := $bitcast.ref.ref($p0);
+  call $p0 := $alloc($mul.ref(16, $zext.i32.i64(1)));
+  assume true;
+  call $p1 := malloc(16);
+  $p2 := $add.ref($add.ref($p0, $mul.ref(0, 16)), $mul.ref(0, 1));
+  $M.0 := $store.ref($M.0, $p2, $p1);
+  call $p3 := malloc(24);
+  $p4 := $add.ref($add.ref($p0, $mul.ref(0, 16)), $mul.ref(8, 1));
+  $M.1 := $store.ref($M.1, $p4, $p3);
+  $p5 := $add.ref($add.ref($p0, $mul.ref(0, 16)), $mul.ref(0, 1));
+  $p6 := $load.ref($M.0, $p5);
+  $p7 := $add.ref($add.ref($p0, $mul.ref(0, 16)), $mul.ref(8, 1));
+  $p8 := $load.ref($M.1, $p7);
+  $i9 := $eq.ref($p6, $p8);
+  assume {:branchcond $i9} true;
+  goto $bb1, $bb2;
+$bb1:
+  assume ($i9 == 1);
+  call free_($p6);
+  call free_($p8);
+  goto $bb3;
+$bb2:
+  assume !(($i9 == 1));
+  goto $bb3;
+$bb3:
+  $p10 := $add.ref($add.ref($p0, $mul.ref(0, 16)), $mul.ref(0, 1));
+  $M.0 := $store.ref($M.0, $p10, $0.ref);
+  $p11 := $add.ref($add.ref($p0, $mul.ref(0, 16)), $mul.ref(8, 1));
+  $M.1 := $store.ref($M.1, $p11, $0.ref);
   $r := 0;
   return;
 }
@@ -25,11 +61,17 @@ procedure  malloc($i0: i64)
 {
   call $r := $malloc($i0);
 }
+const free_: ref;
+axiom (free_ == $sub.ref(0, 4128));
+procedure  free_($p0: ref)
+{
+  call $free($p0);
+}
 const llvm.dbg.value: ref;
-axiom (llvm.dbg.value == $sub.ref(0, 4128));
+axiom (llvm.dbg.value == $sub.ref(0, 5160));
 procedure  llvm.dbg.value($p0: ref, $p1: ref, $p2: ref);
 const __SMACK_static_init: ref;
-axiom (__SMACK_static_init == $sub.ref(0, 5160));
+axiom (__SMACK_static_init == $sub.ref(0, 6192));
 procedure  __SMACK_static_init()
 {
 $bb0:
